

$$f(x_i, x_e, x_n) = \frac{f(x_i, x_j) - f(x_j, x_0)}{x_i - x_0}$$

Ejercicio

x f(x)

1 0

4 1.386294 $C_1/C_2/C_3$ $f(z)$ interpolación es
lines, quadratics y cubics

5 1.609438

Lines | $f_1(x) = \frac{f(x_1) - f(x_0)}{x_1 - x_0} (x - x_0) + f(x_0)$

6 1.751752

$$f_1(z) = \frac{1.386294 - 0}{4 - 1} (z - 1) + 0$$

$$f_1(z) = 0.462098$$

Quadratics

$$f_2(x) = b_0 + b_1(x - x_0) + b_2(x - x_0)(x - x_1)$$

$$b_0 = f(x_0) = 0$$

$$b_1 = \frac{f(x_1) - f(x_0)}{x_1 - x_0} = \frac{1.386294 - 0}{4 - 1} = 0.462098$$

$$b_2 = \frac{f(x_2) - f(x_1)}{x_2 - x_1} - \frac{f(x_1) - f(x_0)}{x_1 - x_0} = \frac{1.609438 - 1.386294}{5 - 4}$$

$$= \frac{1.386294}{4 - 1}$$

$$b_2 = \frac{0.223144 - 0.462098}{4} = -0.059738$$

Norme

$$E_2(x) = 0 + 0.462098(2-1) + (-0.0597385)(2-1)/(2-4)$$

$$E_2(2) = 0 + 0.462098 + 0.119477 = 0.581575$$

Cubics

$$E_3(x) = b_0 + b_1(x-x_0) + b_2(x-x_0)(x-x_1) + b_3(x-x_0)(x-x_1)(x-x_2)$$

$$E_3(x) = f(x_0) + \frac{f(x_2) - f(x_0)}{x_2 - x_0} (x_2 - x_0) + \left(\frac{\frac{f(x_2) - f(x_0)}{x_2 - x_0} - \frac{f(x_1) - f(x_0)}{x_1 - x_0}}{x_2 - x_0} \right) (x_2 - x_0)(x_1 - x_0)$$

$$+ b_3(x-x_0)(x-x_1)(x-x_2)$$

Polinomio de Interpolación de Newton

$$E[x_N, x_{N-1}, x_1, x_0] = \frac{f[x_N, x_{N-1}, x_1] - f[x_N, x_{N-1}, x_0]}{x_N - x_0}$$

$$f[x_3, x_2, x_1, x_0] = \frac{f[x_3, x_2, x_1] - f[x_3, x_2, x_0]}{x_3 - x_0}$$

$$= \frac{\frac{f(x_3, x_2) - f(x_2, x_1)}{x_3 - x_2} - \frac{f(x_3, x_2) - f(x_2, x_0)}{x_3 - x_0}}{x_3 - x_0}$$

$$= \frac{1.791752 - 1.609038}{6-4} - \frac{1.609438 - 1.386294}{6-4} \cdot \frac{1.791752 - 1.609438}{6-1}$$

$$= \frac{1.609438 - 0}{6-1}$$

$$6-1$$

$$= \frac{0.091157 - 0.111572 - 0.0864628 - 0.328876}{5} = -0.07575308$$

$$f_3(z) = 0 + 0.452098(z) + (-0.0557885)/(z-1)(z-4)$$

$$+ (-0.0757)(3)/(z-4)(z-5)$$

$$f_3(z) = 0.12705652$$